Some names refactored. Added descriptions to definitions

poSTVM/poSTVM_state_alt.thy
@@ -41,6 +41,7 @@ definition get_proc_var_by_name :: "stacked_proc_vars \<Rightarrow>  symbolic_va
     | (stacked_proc_var.ProcessVar var) \<Rightarrow> None)"
 declare get_proc_var_by_name_def [simp]
 
+text "Getting var init from program vars by name"
 definition get_prog_var_by_name :: "stacked_prog_vars \<Rightarrow>  symbolic_var \<Rightarrow>  stacked_var_init option" where
   "get_prog_var_by_name vars name =
     (case the (fmlookup vars name) of
@@ -51,6 +52,7 @@ definition get_prog_var_by_name :: "stacked_prog_vars \<Rightarrow>  symbolic_va
     | (stacked_prog_var.ExtVar var) \<Rightarrow>Some var)"
 declare get_prog_var_by_name_def [simp]
 
+text "Getting var init from global vars by name"
 definition get_global_var_by_name :: "stacked_global_vars \<Rightarrow>  symbolic_var \<Rightarrow>  stacked_var_init option" where
   "get_global_var_by_name vars name =
     (case the (fmlookup vars name) of
@@ -61,115 +63,109 @@ declare get_global_var_by_name_def [simp]
 print_theorems
 
 text "Getting current process state from program state"
-definition get_cur_proc_state_by_prog :: "program_state \<Rightarrow> process_state" where
-"get_cur_proc_state_by_prog ps = (case (fmlookup (fst (snd ps)) (snd (snd ps))) of Some (st) \<Rightarrow> st)"
-declare get_cur_proc_state_by_prog_def [simp]
+definition get_cur_procst_from_progst :: "program_state \<Rightarrow> process_state" where
+"get_cur_procst_from_progst ps = (case (fmlookup (fst (snd ps)) (snd (snd ps))) of Some (st) \<Rightarrow> st)"
+declare get_cur_procst_from_progst_def [simp]
 
-definition get_proc_state_by_prog_by_name :: "program_state \<Rightarrow> process_name \<Rightarrow> process_state" where
-"get_proc_state_by_prog_by_name pg pc_name = 
+definition get_procst_from_progst_by_name :: "program_state \<Rightarrow> process_name \<Rightarrow> process_state" where
+"get_procst_from_progst_by_name pg pc_name = 
   (let (_,pc_map,_) = pg in (case (fmlookup pc_map pc_name) of Some st \<Rightarrow> st))"
 
 text "Getting process vars list in current process from program state"
-definition get_cur_proc_vars_from_prog :: "program_state \<Rightarrow>stacked_proc_vars" where 
-  "get_cur_proc_vars_from_prog ps_state = 
-    (let (proc_var_list,st_name,proc_stat,cur_time) = get_cur_proc_state_by_prog ps_state in
+definition get_cur_proc_vars_from_progst :: "program_state \<Rightarrow>stacked_proc_vars" where 
+  "get_cur_proc_vars_from_progst ps_state = 
+    (let (proc_var_list,st_name,proc_stat,cur_time) = get_cur_procst_from_progst ps_state in
       proc_var_list)"
-declare get_cur_proc_vars_from_prog_def [simp]
+declare get_cur_proc_vars_from_progst_def [simp]
 
 text "Getting current program state from model state"
-definition get_cur_prog_state :: "model_state \<Rightarrow> program_state" where
-"get_cur_prog_state st = 
+definition get_cur_progst :: "model_state \<Rightarrow> program_state" where
+"get_cur_progst st = 
   (case st of 
     (ST global_var_decl_list ps_map p_name function_block_decl_list function_decl_list) \<Rightarrow>
       (case (fmlookup ps_map p_name) of 
         Some(p_state) \<Rightarrow> p_state))"
-declare get_cur_prog_state_def [simp]
+declare get_cur_progst_def [simp]
 
 text "Getting current process state name"
 definition get_cur_proc_state_name :: "model_state \<Rightarrow> state_name" where
-"get_cur_proc_state_name st = fst (snd (get_cur_proc_state_by_prog (get_cur_prog_state st)))"
+"get_cur_proc_state_name st = fst (snd (get_cur_procst_from_progst (get_cur_progst st)))"
 declare get_cur_proc_state_name_def [simp]
 
-text "Getting program state by program name from model state"
-definition get_proc_state_by_prog :: "program_state \<Rightarrow> process_name \<Rightarrow> process_state" where
-"get_proc_state_by_prog ps var_name = (case (fmlookup (fst (snd ps)) var_name) of Some (st) \<Rightarrow> st)"
-declare get_proc_state_by_prog_def [simp]
-
 text "Getting process state by process name from model state" 
-definition get_proc_state :: "model_state \<Rightarrow> process_name \<Rightarrow> process_state" where 
-"get_proc_state st var_name =
-  get_proc_state_by_prog (get_cur_prog_state st) var_name"
-declare get_proc_state_def [simp]
+definition get_procst_by_name :: "model_state \<Rightarrow> process_name \<Rightarrow> process_state" where 
+"get_procst_by_name st var_name =
+  get_procst_from_progst_by_name (get_cur_progst st) var_name"
+declare get_procst_by_name_def [simp]
 
-text "Getting process vars list of current process of current program from model state"
+text "Get vars of current process from model state"
 definition get_cur_proc_vars :: "model_state \<Rightarrow> stacked_proc_vars" where
-"get_cur_proc_vars st = get_cur_proc_vars_from_prog (get_cur_prog_state st)"
+"get_cur_proc_vars st = get_cur_proc_vars_from_progst (get_cur_progst st)"
 declare get_cur_proc_vars_def [simp]
 
+text "Get vars of current program from model state"
 definition get_cur_prog_vars :: "model_state \<Rightarrow> stacked_prog_vars" where
-"get_cur_prog_vars st = (let (vars,_,_) = (get_cur_prog_state st) in vars)"
+"get_cur_prog_vars st = (let (vars,_,_) = (get_cur_progst st) in vars)"
 declare get_cur_prog_vars_def [simp]
 
+text "Get global vars"
 definition get_global_vars :: "model_state \<Rightarrow> stacked_global_vars" where
 "get_global_vars st = (case st of (ST vars _ _ _ _) \<Rightarrow> vars)"
 declare get_global_vars_def [simp]
 
-definition get_cur_prog_vars_get :: "model_state \<Rightarrow> stacked_prog_vars" where
-"get_cur_prog_vars_get st = (let (vars,_,_) = (get_cur_prog_state st) in vars)"
-declare get_cur_prog_vars_def [simp]
-
-definition get_var_level_set :: "model_state \<Rightarrow> symbolic_var \<Rightarrow> var_level" where
-"get_var_level_set st var_name =
+text "Getting level of var by name for setting purpose"
+definition get_var_level_by_name_for_set :: "model_state \<Rightarrow> symbolic_var \<Rightarrow> var_level" where
+"get_var_level_by_name_for_set st var_name =
   (case (fmlookup (get_global_vars st) var_name) of
     Some _ \<Rightarrow> var_level.Global
   | None \<Rightarrow> (case (fmlookup (get_cur_prog_vars st) var_name) of
               Some _ \<Rightarrow> var_level.Program
             | None \<Rightarrow> (case (fmlookup (get_cur_proc_vars st) var_name) of
                         Some _ \<Rightarrow> var_level.Process)))"
-declare get_var_level_set_def [simp]
+declare get_var_level_by_name_for_set_def [simp]
 
-definition get_var_level_get :: "model_state \<Rightarrow> symbolic_var \<Rightarrow> var_level" where
-"get_var_level_get st var_name =
+text "Getting level of var by name for getting purpose"
+definition get_var_level_by_name_for_get :: "model_state \<Rightarrow> symbolic_var \<Rightarrow> var_level" where
+"get_var_level_by_name_for_get st var_name =
   (case (fmlookup (get_global_vars st) var_name) of
     Some _ \<Rightarrow> var_level.Global
   | None \<Rightarrow> (case (fmlookup (get_cur_prog_vars st) var_name) of
               Some _ \<Rightarrow> var_level.Program
             | None \<Rightarrow> (case (fmlookup (get_cur_proc_vars st) var_name) of
                         Some _ \<Rightarrow> var_level.Process)))"
-declare get_var_level_get_def [simp]
+declare get_var_level_by_name_for_get_def [simp]
 
 text "Getting variable init by name from model state"
-definition get_cur_var_by_name :: "model_state \<Rightarrow> symbolic_var \<Rightarrow> stacked_var_init" where
-"get_cur_var_by_name st var_name = 
-  (case (get_var_level_get st var_name) of
+definition get_cur_var_init_by_name :: "model_state \<Rightarrow> symbolic_var \<Rightarrow> stacked_var_init" where
+"get_cur_var_init_by_name st var_name = 
+  (case (get_var_level_by_name_for_get st var_name) of
     var_level.Global \<Rightarrow> the (get_global_var_by_name (get_global_vars st) var_name)
   | var_level.Program \<Rightarrow> the (get_prog_var_by_name (get_cur_prog_vars st) var_name)
   | var_level.Process \<Rightarrow> the (get_proc_var_by_name (get_cur_proc_vars st) var_name))"
-declare get_cur_var_by_name_def [simp]
-
+declare get_cur_var_init_by_name_def [simp]
 
 text "Getting symbolic variable value by name from model state"
-definition get_symbvar_by_name :: "model_state \<Rightarrow> symbolic_var \<Rightarrow> basic_post_type" where
-"get_symbvar_by_name st var_name = 
-  (case (get_cur_var_by_name st var_name) of
+definition get_cur_symbvar_by_name :: "model_state \<Rightarrow> symbolic_var \<Rightarrow> basic_post_type" where
+"get_cur_symbvar_by_name st var_name = 
+  (case (get_cur_var_init_by_name st var_name) of
     (stacked_var_init.Symbolic val opt) \<Rightarrow> val)"
-declare get_symbvar_by_name_def [simp]
+declare get_cur_symbvar_by_name_def [simp]
 
-text "Getting values from list of values"
-definition get_bval_from_list :: "basic_post_type list \<Rightarrow> basic_post_type \<Rightarrow> basic_post_type" where
-"get_bval_from_list bl pos =
+text "Getting value from list of values by basic_post_type position"
+definition get_val_from_list_by_basic :: "'a list \<Rightarrow> basic_post_type \<Rightarrow> 'a" where
+"get_val_from_list_by_basic bl pos =
   (case pos of
     (basic_post_type.Nat val) \<Rightarrow> (nth bl val) |
     (basic_post_type.Int val) \<Rightarrow> (nth bl (nat val)))"
-declare get_bval_from_list_def [simp]
+declare get_val_from_list_by_basic_def [simp]
 
 text "Getting array variable single values by name and absolute position from model state"
-definition get_arvar_by_name :: "model_state \<Rightarrow> symbolic_var \<Rightarrow> basic_post_type \<Rightarrow> basic_post_type" where
-"get_arvar_by_name st var_name pos =
-  (case (get_cur_var_by_name st var_name) of
+definition get_cur_arvar_by_name_by_pos :: "model_state \<Rightarrow> symbolic_var \<Rightarrow> basic_post_type \<Rightarrow> basic_post_type" where
+"get_cur_arvar_by_name_by_pos st var_name pos =
+  (case (get_cur_var_init_by_name st var_name) of
     (stacked_var_init.Array (stacked_array_interval.Int val1 val2) values  opt) \<Rightarrow>
-      (get_bval_from_list values (basic_post_type_sum (basic_post_type.Int val1) pos)))"
-declare get_arvar_by_name_def [simp]
+      (get_val_from_list_by_basic values (basic_post_type_sum (basic_post_type.Int val1) pos)))"
+declare get_cur_arvar_by_name_by_pos_def [simp]
 
 text "Setting in process vars list new var init value by name"
 definition set_symbvar_in_proc_vars :: "(stacked_proc_vars) \<Rightarrow>  symbolic_var \<Rightarrow> stacked_var_init \<Rightarrow> stacked_proc_vars" where
@@ -181,8 +177,9 @@ definition set_symbvar_in_proc_vars :: "(stacked_proc_vars) \<Rightarrow>  symbo
   | (stacked_proc_var.OutVar var) \<Rightarrow> (fmupd name (stacked_proc_var.OutVar val) vars))"
 declare set_symbvar_in_proc_vars_def [simp]
 
-definition set_symbvar_in_cur_proc_vars :: "model_state \<Rightarrow> symbolic_var \<Rightarrow> stacked_var_init \<Rightarrow> model_state" where
-"set_symbvar_in_cur_proc_vars st var_name val = 
+text "Setting symbolic var in current process in model state"
+definition set_cur_proc_symbvar :: "model_state \<Rightarrow> symbolic_var \<Rightarrow> stacked_var_init \<Rightarrow> model_state" where
+"set_cur_proc_symbvar st var_name val = 
   (case st of (ST global_vars pg_map pg_name  f1 f2) \<Rightarrow>
     (let (prog_vars,pc_map,pc_name) = the (fmlookup pg_map pg_name);
          (proc_vars,v1,v2,v3,v4,v5) = the (fmlookup pc_map pc_name)
@@ -200,8 +197,9 @@ definition set_symbvar_in_cur_proc_vars :: "model_state \<Rightarrow> symbolic_v
           pg_name
          f1
          f2)))"
-declare set_symbvar_in_cur_proc_vars_def [simp]
+declare set_cur_proc_symbvar_def [simp]
 
+text "Setting symbolic var in program vars"
 definition set_symbvar_in_prog_vars :: "stacked_prog_vars \<Rightarrow> symbolic_var \<Rightarrow> stacked_var_init \<Rightarrow> stacked_prog_vars" where
 "set_symbvar_in_prog_vars vars name val= 
   (case the (fmlookup vars name) of
@@ -212,8 +210,9 @@ definition set_symbvar_in_prog_vars :: "stacked_prog_vars \<Rightarrow> symbolic
   | (stacked_prog_var.ExtVar var) \<Rightarrow> (fmupd name (stacked_prog_var.ExtVar val) vars))"
 declare set_symbvar_in_prog_vars_def [simp]
 
-definition set_symbvar_in_cur_prog_vars :: "model_state \<Rightarrow> symbolic_var \<Rightarrow> stacked_var_init \<Rightarrow> model_state" where
-"set_symbvar_in_cur_prog_vars st var_name val = 
+text "Setting symbolic var in current program in model state"
+definition set_cur_prog_symbvar :: "model_state \<Rightarrow> symbolic_var \<Rightarrow> stacked_var_init \<Rightarrow> model_state" where
+"set_cur_prog_symbvar st var_name val = 
   (case st of (ST global_vars pg_map pg_name  f1 f2) \<Rightarrow>
     (let (prog_vars,pc_map,pc_name) = the (fmlookup pg_map pg_name)
      in (ST
@@ -227,61 +226,63 @@ definition set_symbvar_in_cur_prog_vars :: "model_state \<Rightarrow> symbolic_v
          pg_name
          f1
          f2)))"
-declare set_symbvar_in_cur_prog_vars_def [simp]
+declare set_cur_prog_symbvar_def [simp]
 
+text "Setting symbolic var in global vars"
 definition set_symbvar_in_global_vars :: "stacked_global_vars \<Rightarrow> symbolic_var \<Rightarrow> stacked_var_init \<Rightarrow> stacked_global_vars" where
 "set_symbvar_in_global_vars vars name val= 
   (case the (fmlookup vars name) of
     (stacked_global_var.Var var) \<Rightarrow> (fmupd name (stacked_global_var.Var val) vars))"
 declare set_symbvar_in_global_vars_def [simp]
 
-definition set_symbvar_in_cur_global_vars :: "model_state \<Rightarrow> symbolic_var \<Rightarrow> stacked_var_init \<Rightarrow> model_state" where
-"set_symbvar_in_cur_global_vars st var_name val = 
+text "Setting global symbolic var in model state"
+definition set_global_symbvar :: "model_state \<Rightarrow> symbolic_var \<Rightarrow> stacked_var_init \<Rightarrow> model_state" where
+"set_global_symbvar st var_name val = 
   (case st of (ST global_vars pg_map pg_name  funcs funblocks) \<Rightarrow>
     (ST
      (set_symbvar_in_global_vars global_vars var_name val) 
      pg_map pg_name 
      funcs
      funblocks))"
-declare set_symbvar_in_cur_global_vars_def [simp]
+declare set_global_symbvar_def [simp]
 
 text "Setting in model state new symbolic var value by name"
 definition set_symbvar :: "model_state \<Rightarrow> symbolic_var \<Rightarrow> basic_post_type => model_state" where
 "set_symbvar st var_name value =
   (let val = (stacked_var_init.Symbolic value None) in
-  (case (get_var_level_set st var_name) of
-    var_level.Global \<Rightarrow> (set_symbvar_in_cur_global_vars st var_name val)
-  | var_level.Program \<Rightarrow> (set_symbvar_in_cur_prog_vars st var_name val)
-  | var_level.Process \<Rightarrow> (set_symbvar_in_cur_proc_vars st var_name val)))"
+  (case (get_var_level_by_name_for_set st var_name) of
+    var_level.Global \<Rightarrow> (set_global_symbvar st var_name val)
+  | var_level.Program \<Rightarrow> (set_cur_prog_symbvar st var_name val)
+  | var_level.Process \<Rightarrow> (set_cur_proc_symbvar st var_name val)))"
 declare set_symbvar_def [simp]
 
-text "Setting new val to list in position"
-definition set_bval_to_list :: "basic_post_type list \<Rightarrow> basic_post_type \<Rightarrow> basic_post_type \<Rightarrow> basic_post_type list" where
-"set_bval_to_list l pos new_val = 
+text "Setting new val to list in basic_post_type position"
+definition set_val_to_list_by_basic :: "'a list \<Rightarrow> basic_post_type \<Rightarrow> 'a \<Rightarrow> 'a list" where
+"set_val_to_list_by_basic l pos new_val = 
   (case pos of 
     basic_post_type.Nat pos \<Rightarrow> (list_update l pos new_val) |
     basic_post_type.Int pos \<Rightarrow> (list_update l (nat pos) new_val))"
-declare set_bval_to_list_def [simp]
+declare set_val_to_list_by_basic_def [simp]
 
 text "Setting in model state new array variable single values by name and absolute position"
 definition set_arvar :: "model_state \<Rightarrow> symbolic_var \<Rightarrow> basic_post_type \<Rightarrow> basic_post_type \<Rightarrow>  model_state" where
 "set_arvar st var_name pos value =
-  (case (get_cur_var_by_name st var_name) of
+  (case (get_cur_var_init_by_name st var_name) of
     (stacked_var_init.Array (stacked_array_interval.Int val1 val2) values  opt) \<Rightarrow> 
       (let val = (stacked_var_init.Array 
                   (stacked_array_interval.Int val1 val2)
-                  (set_bval_to_list values (basic_post_type_sum (basic_post_type.Int val1) pos) value)
+                  (set_val_to_list_by_basic values (basic_post_type_sum (basic_post_type.Int val1) pos) value)
                   opt) in 
-  (case (get_var_level_set st var_name) of
-    var_level.Global \<Rightarrow> (set_symbvar_in_cur_global_vars st var_name val)
-  | var_level.Program \<Rightarrow> (set_symbvar_in_cur_prog_vars st var_name val)
-  | var_level.Process \<Rightarrow> (set_symbvar_in_cur_proc_vars st var_name val)))) "
+  (case (get_var_level_by_name_for_set st var_name) of
+    var_level.Global \<Rightarrow> (set_global_symbvar st var_name val)
+  | var_level.Program \<Rightarrow> (set_cur_prog_symbvar st var_name val)
+  | var_level.Process \<Rightarrow> (set_cur_proc_symbvar st var_name val)))) "
 declare set_arvar_def [simp]
 
 text "Compare process status and estimated status"
 definition check_proc_status :: "model_state \<Rightarrow> process_name \<Rightarrow> proc_status \<Rightarrow> basic_post_type" where
 "check_proc_status st name proc_stat = 
-  (let (_,_,_,_, cur_proc_stat,_) = (get_proc_state st name) 
+  (let (_,_,_,_, cur_proc_stat,_) = (get_procst_by_name st name) 
     in (basic_post_type.Bool (proc_status_is cur_proc_stat proc_stat)))"
 declare check_proc_status_def [simp]
 
@@ -289,7 +290,7 @@ text "Setting current process name in current program"
 definition set_cur_proc_name :: "model_state \<Rightarrow> process_name \<Rightarrow> model_state" where
 "set_cur_proc_name st name = 
   (case st of (ST g_list pg_map pg_name f1 f2) \<Rightarrow>
-      (let (var_list, p_map,p_name) = (get_cur_prog_state st)
+      (let (var_list, p_map,p_name) = (get_cur_progst st)
            
         in (ST g_list 
           (fmupd 
@@ -308,12 +309,12 @@ definition set_cur_prog_name :: "model_state \<Rightarrow> program_name \<Righta
 declare set_cur_prog_name_def [simp]
 
 text "Resetting timer in current process in model state"
-definition reset_timer :: "model_state \<Rightarrow> model_state" where
-"reset_timer st = 
+definition reset_cur_timer :: "model_state \<Rightarrow> model_state" where
+"reset_cur_timer st = 
   (case st of
     (ST g_list pg_map pg_name fb_list f_list) \<Rightarrow>
-      (let (var_list, p_map,p_name) = (get_cur_prog_state st);
-           (process_vars, current_state, next_state, state_names, process_status, t) = (get_cur_proc_state_by_prog (var_list,p_map,p_name))
+      (let (var_list, p_map,p_name) = (get_cur_progst st);
+           (process_vars, current_state, next_state, state_names, process_status, t) = (get_cur_procst_from_progst (var_list,p_map,p_name))
         in (ST g_list 
           (fmupd 
               pg_name 
@@ -323,15 +324,15 @@ definition reset_timer :: "model_state \<Rightarrow> model_state" where
                  p_map),p_name)
               pg_map) 
             pg_name fb_list f_list)))"
-declare reset_timer_def [simp]
+declare reset_cur_timer_def [simp]
 
 text "Stopping process by name in model state"
 definition stop_process :: "model_state \<Rightarrow> process_name \<Rightarrow> model_state" where
 "stop_process st target_proc_name =
     (case st of
     (ST g_list pg_map pg_name fb_list f_list) \<Rightarrow>
-      (let (var_list, p_map,p_name) = (get_cur_prog_state st);
-           (process_vars, current_state, next_state, state_names, process_status, t) = (get_proc_state_by_prog_by_name (var_list,p_map,p_name) target_proc_name)
+      (let (var_list, p_map,p_name) = (get_cur_progst st);
+           (process_vars, current_state, next_state, state_names, process_status, t) = (get_procst_from_progst_by_name (var_list,p_map,p_name) target_proc_name)
         in (ST g_list 
           (fmupd 
               pg_name 
@@ -344,12 +345,12 @@ definition stop_process :: "model_state \<Rightarrow> process_name \<Rightarrow>
 declare stop_process_def [simp]
 
 text "Stopping current process in model state"
-definition stop_same_process :: "model_state  \<Rightarrow> model_state" where
-"stop_same_process st =
+definition stop_cur_process :: "model_state  \<Rightarrow> model_state" where
+"stop_cur_process st =
   (case st of
     (ST g_list pg_map pg_name fb_list f_list) \<Rightarrow>
-      (let (var_list, p_map,p_name) = (get_cur_prog_state st);
-           (process_vars, current_state, next_state, state_names, process_status, t) = (get_proc_state_by_prog_by_name (var_list,p_map,p_name) p_name)
+      (let (var_list, p_map,p_name) = (get_cur_progst st);
+           (process_vars, current_state, next_state, state_names, process_status, t) = (get_procst_from_progst_by_name (var_list,p_map,p_name) p_name)
         in (ST g_list 
           (fmupd 
               pg_name 
@@ -359,15 +360,15 @@ definition stop_same_process :: "model_state  \<Rightarrow> model_state" where
                  p_map),p_name)
               pg_map) 
             pg_name fb_list f_list)))"
-declare stop_same_process_def [simp]
+declare stop_cur_process_def [simp]
 
 text "Erroring process by name in model state"
 definition error_process :: "model_state \<Rightarrow> process_name \<Rightarrow> model_state" where
 "error_process st target_proc_name =
    (case st of
     (ST g_list pg_map pg_name fb_list f_list) \<Rightarrow>
-      (let (var_list, p_map,p_name) = (get_cur_prog_state st);
-           (process_vars, current_state, next_state, state_names, process_status, t) = (get_proc_state_by_prog_by_name (var_list,p_map,p_name) target_proc_name)
+      (let (var_list, p_map,p_name) = (get_cur_progst st);
+           (process_vars, current_state, next_state, state_names, process_status, t) = (get_procst_from_progst_by_name (var_list,p_map,p_name) target_proc_name)
         in (ST g_list 
           (fmupd 
               pg_name 
@@ -380,12 +381,12 @@ definition error_process :: "model_state \<Rightarrow> process_name \<Rightarrow
 declare error_process_def [simp]
 
 text "Erroring current process in model state"
-definition error_same_process :: "model_state \<Rightarrow> model_state" where
-"error_same_process st=
+definition error_cur_process :: "model_state \<Rightarrow> model_state" where
+"error_cur_process st=
    (case st of
     (ST g_list pg_map pg_name fb_list f_list) \<Rightarrow>
-      (let (var_list, p_map,p_name) = (get_cur_prog_state st);
-           (process_vars, current_state, next_state, state_names, process_status, t) = (get_proc_state_by_prog_by_name (var_list,p_map,p_name) p_name)
+      (let (var_list, p_map,p_name) = (get_cur_progst st);
+           (process_vars, current_state, next_state, state_names, process_status, t) = (get_procst_from_progst_by_name (var_list,p_map,p_name) p_name)
         in (ST g_list 
           (fmupd 
               pg_name 
@@ -395,15 +396,15 @@ definition error_same_process :: "model_state \<Rightarrow> model_state" where
                  p_map),p_name)
               pg_map) 
             pg_name fb_list f_list)))"
-declare error_same_process_def [simp]
+declare error_cur_process_def [simp]
 
 text "Resetting process by name in model state"
 definition reset_process :: "model_state \<Rightarrow> process_name \<Rightarrow> model_state" where
 "reset_process st target_proc_name =
  (case st of
     (ST g_list pg_map pg_name fb_list f_list) \<Rightarrow>
-      (let (var_list, p_map,p_name) = (get_cur_prog_state st);
-           (process_vars, current_state, next_state, state_names, process_status, t) = (get_proc_state_by_prog_by_name (var_list,p_map,p_name) target_proc_name)
+      (let (var_list, p_map,p_name) = (get_cur_progst st);
+           (process_vars, current_state, next_state, state_names, process_status, t) = (get_procst_from_progst_by_name (var_list,p_map,p_name) target_proc_name)
         in (ST g_list 
           (fmupd 
               pg_name 
@@ -416,12 +417,12 @@ definition reset_process :: "model_state \<Rightarrow> process_name \<Rightarrow
 declare reset_process_def [simp]
 
 text "Resetting current process in model state"
-definition reset_same_process :: "model_state \<Rightarrow> model_state" where
-"reset_same_process st  =
+definition reset_cur_process :: "model_state \<Rightarrow> model_state" where
+"reset_cur_process st  =
  (case st of
     (ST g_list pg_map pg_name fb_list f_list) \<Rightarrow>
-      (let (var_list, p_map,p_name) = (get_cur_prog_state st);
-           (process_vars, current_state, next_state, state_names, process_status, t) = (get_proc_state_by_prog_by_name (var_list,p_map,p_name) p_name)
+      (let (var_list, p_map,p_name) = (get_cur_progst st);
+           (process_vars, current_state, next_state, state_names, process_status, t) = (get_procst_from_progst_by_name (var_list,p_map,p_name) p_name)
         in (ST g_list 
           (fmupd 
               pg_name 
@@ -431,14 +432,14 @@ definition reset_same_process :: "model_state \<Rightarrow> model_state" where
                  p_map),p_name)
               pg_map) 
             pg_name fb_list f_list)))"
-declare reset_same_process_def [simp]
+declare reset_cur_process_def [simp]
 
-definition inactive_same_process :: "model_state \<Rightarrow> model_state" where
-"inactive_same_process st =
+definition inactive_cur_process :: "model_state \<Rightarrow> model_state" where
+"inactive_cur_process st =
   (case st of
     (ST g_list pg_map pg_name fb_list f_list) \<Rightarrow>
-      (let (var_list, p_map,p_name) = (get_cur_prog_state st);
-           (process_vars, current_state, next_state, state_names, process_status, t) = (get_proc_state_by_prog_by_name (var_list,p_map,p_name) p_name)
+      (let (var_list, p_map,p_name) = (get_cur_progst st);
+           (process_vars, current_state, next_state, state_names, process_status, t) = (get_procst_from_progst_by_name (var_list,p_map,p_name) p_name)
         in (ST g_list 
           (fmupd 
               pg_name 
@@ -448,14 +449,14 @@ definition inactive_same_process :: "model_state \<Rightarrow> model_state" wher
                  p_map),p_name)
               pg_map) 
             pg_name fb_list f_list)))"
-declare inactive_same_process_def [simp]
+declare inactive_cur_process_def [simp]
 
 definition inactive_process :: "model_state \<Rightarrow> process_name \<Rightarrow> model_state" where
 "inactive_process st target_proc_name =
    (case st of
     (ST g_list pg_map pg_name fb_list f_list) \<Rightarrow>
-      (let (var_list, p_map,p_name) = (get_cur_prog_state st);
-           (process_vars, current_state, next_state, state_names, process_status, t) = (get_proc_state_by_prog_by_name (var_list,p_map,p_name) target_proc_name)
+      (let (var_list, p_map,p_name) = (get_cur_progst st);
+           (process_vars, current_state, next_state, state_names, process_status, t) = (get_procst_from_progst_by_name (var_list,p_map,p_name) target_proc_name)
         in (ST g_list 
           (fmupd 
               pg_name 
@@ -472,8 +473,8 @@ definition set_state :: "model_state \<Rightarrow> state_name \<Rightarrow> mode
 "set_state st st_name = 
   (case st of
     (ST g_list pg_map pg_name fb_list f_list) \<Rightarrow>
-      (let (var_list, p_map,p_name) = (get_cur_prog_state st);
-           (process_vars, current_state, next_state, state_names, process_status, t) = (get_proc_state_by_prog_by_name (var_list,p_map,p_name) p_name)
+      (let (var_list, p_map,p_name) = (get_cur_progst st);
+           (process_vars, current_state, next_state, state_names, process_status, t) = (get_procst_from_progst_by_name (var_list,p_map,p_name) p_name)
         in (ST g_list 
           (fmupd 
               pg_name 
@@ -485,35 +486,39 @@ definition set_state :: "model_state \<Rightarrow> state_name \<Rightarrow> mode
             pg_name fb_list f_list)))"
 declare set_state_def [simp]
 
-definition get_timeout :: "model_state \<Rightarrow> stacked_state \<Rightarrow> time" where
-"get_timeout st ss =
+text "Getting timeout of state"
+definition get_state_timeout :: "model_state \<Rightarrow> stacked_state \<Rightarrow> time" where
+"get_state_timeout st ss =
   (case ss of
     (_,_,_, Some (timeout.Const t _)) => basic_to_time (const_to_basic t)
-  | (_,_,_, Some (timeout.SymbolicVar var_name _)) => basic_to_time (get_symbvar_by_name st var_name))"
-declare get_timeout_def [simp]
+  | (_,_,_, Some (timeout.SymbolicVar var_name _)) => basic_to_time (get_cur_symbvar_by_name st var_name))"
+declare get_state_timeout_def [simp]
 
-definition get_same_time :: "model_state \<Rightarrow> time" where
-"get_same_time st = 
+text "Getting time of current process"
+definition get_cur_time :: "model_state \<Rightarrow> time" where
+"get_cur_time st = 
  (case st of (ST global_var_decl_list pg_map p_name function_block_decl_list function_decl_list) \<Rightarrow>
     (let (var_list,proc_map, proc_name) = (case (fmlookup pg_map p_name) of Some(p_state) \<Rightarrow> p_state);
         (proc_vars,st_name,next_state,state_names, proc_stat, cur_time) = (case (fmlookup proc_map proc_name) of Some(proc_state) \<Rightarrow> proc_state)
     in cur_time)) "
-declare get_same_time_def [simp]
+declare get_cur_time_def [simp]
 
-definition get_time :: "model_state \<Rightarrow> process_name \<Rightarrow> time" where
-"get_time st proc_name= 
+text "Getting time of process by name"
+definition get_process_time_by_name :: "model_state \<Rightarrow> process_name \<Rightarrow> time" where
+"get_process_time_by_name st proc_name= 
  (case st of (ST global_var_decl_list pg_map pg_name  function_block_decl_list function_decl_list) \<Rightarrow>
     (let (var_list,proc_map, _) = (case (fmlookup pg_map pg_name) of Some(p_state) \<Rightarrow> p_state);
         ((proc_var_list),st_name,next_state,state_names, proc_stat, cur_time) = (case (fmlookup proc_map proc_name) of Some(proc_state) \<Rightarrow> proc_state)
   in cur_time)) "
-declare get_time_def [simp]
+declare get_process_time_by_name_def [simp]
 
+text "Getting name of next state"
 primrec get_next_state_name :: "state_name list \<Rightarrow> state_name \<Rightarrow> state_name" where
 "get_next_state_name (st_name#other) name =
   (if (st_name = name) then (hd other) else get_next_state_name other name)"
-print_theorems
 declare get_next_state_name.simps [simp]
 
+text "Setting next state name in next state"
 definition set_next_state_next :: "model_state \<Rightarrow> model_state" where
 "set_next_state_next st = 
  (case st of (ST global_var_decl_list pg_map pg_name function_block_decl_list function_decl_list) \<Rightarrow>
@@ -536,6 +541,7 @@ definition set_next_state_next :: "model_state \<Rightarrow> model_state" where
         function_decl_list))) " 
 declare set_next_state_next_def [simp]
 
+text "Setting current state into next state"
 definition set_into_next_state :: "model_state \<Rightarrow> model_state" where
 "set_into_next_state st = 
  (case st of (ST global_var_decl_list pg_map pg_name  function_block_decl_list function_decl_list) \<Rightarrow>
@@ -557,6 +563,7 @@ definition set_into_next_state :: "model_state \<Rightarrow> model_state" where
         function_decl_list))) " 
 declare set_into_next_state_def [simp]
 
+text "Extract timeout stmt if cur process time more than timeout "
 definition extr_timeout_stmt :: "model_state \<Rightarrow> timeout \<Rightarrow> (stmt option)" where
 "extr_timeout_stmt st timeo = 
   (case st of (ST global_var_decl_list pg_map pg_name function_block_decl_list function_decl_list) \<Rightarrow>
@@ -565,7 +572,7 @@ definition extr_timeout_stmt :: "model_state \<Rightarrow> timeout \<Rightarrow>
                                     Some(proc_state) \<Rightarrow> proc_state) 
   in (case timeo of
        (timeout.Const c stm) \<Rightarrow>  (if (time_less (basic_to_time (const_to_basic c)) cur_time) then (Some stm) else None)
-     | (timeout.SymbolicVar sv stm) \<Rightarrow> (if (time_less (basic_to_time (get_symbvar_by_name st sv)) cur_time) then (Some stm) else None))))"
+     | (timeout.SymbolicVar sv stm) \<Rightarrow> (if (time_less (basic_to_time (get_cur_symbvar_by_name st sv)) cur_time) then (Some stm) else None))))"
 declare extr_timeout_stmt_def [simp]
 
 text "Gather out and inout vars from process vars"
@@ -616,6 +623,7 @@ definition update_processes_in_vars :: "((process_name,process_state) fmap) \<Ri
     proc_map)"
 declare update_processes_in_vars_def [simp]
 
+text "Distribution of process out vars values"
 definition process_vars_distribution :: "model_state \<Rightarrow> model_state" where
 "process_vars_distribution st = 
   (case st of (ST global_var_decl_list pg_map pg_name f1 f2) \<Rightarrow>
@@ -679,6 +687,7 @@ definition update_programs_in_vars :: "((program_name,program_state) fmap) \<Rig
     prog_map)"
 declare update_programs_in_vars_def [simp]
 
+text "Distribution of program out vars values"
 definition program_vars_distribution :: "model_state \<Rightarrow> model_state" where
 "program_vars_distribution st = 
   (case st of (ST global_var_decl_list ps_map p_name f1 f2) \<Rightarrow>
@@ -688,26 +697,7 @@ definition program_vars_distribution :: "model_state \<Rightarrow> model_state" 
       p_name f1 f2)))"
 declare program_vars_distribution_def [simp]
 
-(*
-definition add_time_to_processes :: "model_state \<Rightarrow> time \<Rightarrow> model_state" where
-"add_time_to_processes st t = 
-  (case st of (ST global_var_decl_list (ps_map,p_name) function_block_decl_list function_decl_list) \<Rightarrow>
-    (let (var_list,proc_map, proc_name) = (case (fmlookup ps_map p_name) of Some(p_state) \<Rightarrow> p_state)
-  in (ST 
-        global_var_decl_list 
-        ((fmupd 
-            p_name
-            (var_list,
-              (fmmap 
-              (\<lambda>(v1,v2,v3,v4,v5,v6).(v1,v2,v3,v4,v5,time_sum v6 t))
-              proc_map), 
-              proc_name) 
-            ps_map),
-          p_name) 
-        function_block_decl_list 
-        function_decl_list)))"
-declare add_time_to_processes_def [simp]
-*)
+text "Incrementing active processes time by time step"
 definition add_time_to_active_processes :: "model_state \<Rightarrow> time \<Rightarrow> model_state" where
 "add_time_to_active_processes st t = 
   (case st of (ST global_var_decl_list pg_map pg_name function_block_decl_list function_decl_list) \<Rightarrow>
@@ -728,6 +718,7 @@ definition add_time_to_active_processes :: "model_state \<Rightarrow> time \<Rig
         function_decl_list)))"
 declare add_time_to_active_processes_def [simp]
 
+text "Checking is process active by name"
 definition is_process_active :: "model_state \<Rightarrow> process_name \<Rightarrow> bool" where
 "is_process_active st name = 
   (case st of (ST global_var_decl_list pg_map pg_name function_block_decl_list function_decl_list) \<Rightarrow>
@@ -736,36 +727,10 @@ definition is_process_active :: "model_state \<Rightarrow> process_name \<Righta
     in (proc_status_is status proc_status.Active)))"
 declare is_process_active_def [simp]
 
-definition filter_active_processes :: "model_state \<Rightarrow> stacked_process list \<Rightarrow> stacked_process list" where
-"filter_active_processes st p_list = (filter (\<lambda>(name,_,_). is_process_active st name) p_list)"
-declare filter_active_processes_def [simp]
-
-(*
-text "Process state in form of process vars list, current state, next_state, list of states, process status, process time"
-type_synonym process_state = "stacked_proc_vars * 
-                              state_name * 
-                              state_name * 
-                              (state_name list) * 
-                              proc_status * 
-                              current_time"
-
-text "Program state in form of program vars list, processes map, current process"
-type_synonym program_state ="stacked_prog_vars * 
-                             ((process_name,process_state) fmap) * 
-                             process_name"
-
-text "Model state in form of global vars, programs map, current program, function blocks list, functions list"
-datatype model_state = ST 
-                       stacked_global_vars  
-                       "((program_name,program_state) fmap * 
-                       program_name)"  
-                       "(function_block_decl list)"  
-                       "(function_decl list)"
-*)
-
-definition get_func :: "model_state \<Rightarrow> func_name \<Rightarrow> stacked_func" where
-"get_func st name = 
+text "Getting function body by name"
+definition get_func_by_name :: "model_state \<Rightarrow> func_name \<Rightarrow> stacked_func" where
+"get_func_by_name st name = 
   (case st of (ST _ _ _ _ f_map) \<Rightarrow> the (fmlookup f_map name))"
-declare get_func_def [simp] 
+declare get_func_by_name_def [simp] 
 
 end
